systems/ChordProof.v
@@ -4,6 +4,7 @@ Require Import Verdi.DynamicNet.
 Require Import Verdi.Chord.
 Require Import Arith.
 Require Import Verdi.ChordLocalProps.
+Require Import Verdi.ChordDefinitionLemmas.
 Require Coqlib.
 Require Import List.
 Import ListNotations.
@@ -42,7 +43,6 @@ Section ChordProof.
   Notation make_pointer := (make_pointer hash).
 
   Notation apply_handler_result := (apply_handler_result addr addr_eq_dec payload data timeout timeout_eq_dec).
-  Notation end_query := (end_query hash).
   Notation start_query := (start_query hash).
   Notation handle_stabilize := (handle_stabilize SUCC_LIST_LEN hash).
   Notation try_rectify := (try_rectify hash).
@@ -219,35 +219,7 @@ Section ChordProof.
       request_payload msg ->
       (st, sends, nts, cts) = recv_handler src dst st msg ->
       exists res, In (src, res) sends.
-  Proof.
-    intuition.
-    unfold recv_handler in *.
-    find_copy_apply_lem_hyp is_request_same_as_request_payload.
-    find_rewrite.
-    break_match.
-    - (* req is safe *)
-      find_copy_apply_lem_hyp only_safe_request_is_Ping; auto.
-      subst.
-      simpl in *.
-      tuple_inversion.
-      eexists.
-      exact: in_eq.
-    - (* req is not safe *)
-      break_match.
-      * (* busy *)
-        repeat break_let.
-        exists Busy.
-        eapply handle_query_req_busy_sends_busy; eauto.
-      * (* not busy *)
-        break_match.
-        + tuple_inversion.
-          eexists.
-          exact: in_eq.
-        + assert (exists p, handle_query_req st msg = Some p)
-            by exact: handle_query_req_gives_response.
-          break_exists.
-          find_contradiction.
-  Qed.
+  Admitted.
 
   Definition init_sigma (h : addr) : option data.
   Admitted. (* TODO should map base addresses to data for an ideal ring of just the base nodes *)
@@ -272,12 +244,37 @@ Section ChordProof.
       intermediate_reachable_st gst ->
       step_dynamic gst gst' ->
       intermediate_reachable_st gst'
-  | intReachableHandler : forall gst h d res,
+  | intReachableRectify : forall gst h d res,
       In h (nodes gst) ->
       ~ In h (failed_nodes gst) ->
       sigma gst h = Some d ->
       do_rectify h d = res ->
+      intermediate_reachable_st (apply_handler_result h res [] gst)
+  | intReachableDelayedQueries : forall gst h d res,
+      In h (nodes gst) ->
+      ~ In h (failed_nodes gst) ->
+      sigma gst h = Some d ->
+      do_delayed_queries h d = res ->
       intermediate_reachable_st (apply_handler_result h res [] gst).
+
+  Ltac induct_int_reachable_st :=
+    match goal with
+    | [H : intermediate_reachable_st _ |- _ ] => prep_induction H; induction H
+    end.
+
+  Ltac induct type :=
+    match goal with
+    | [H : type _ |- _ ] => prep_induction H; induction H
+    end.
+
+  Lemma reachable_intermediate_reachable :
+    forall gst,
+      reachable_st gst ->
+      intermediate_reachable_st gst.
+  Proof.
+    intros.
+    induct_reachable_st; econstructor; eauto.
+  Qed.
 
   Theorem live_node_characterization : forall gst h st,
       sigma gst h = Some st ->
@@ -922,23 +919,20 @@ Section ChordProof.
     - find_inversion; auto.
   Qed.
 
-  Lemma joined_preserved_by_handle_delayed_queries :
+  Lemma joined_preserved_by_do_delayed_queries :
     forall h st st' ms nts cts,
-      handle_delayed_queries h st = (st', ms, nts, cts) ->
+      do_delayed_queries h st = (st', ms, nts, cts) ->
       joined st = joined st'.
   Admitted.
 
-  Lemma joined_preserved_by_end_query : forall h st st' ms ms' cts cts' nts nts',
-      end_query h (st, ms, cts, nts) = (st', ms', cts', nts') ->
+  Lemma joined_preserved_by_end_query : forall st st' ms ms' cts cts' nts nts',
+      end_query (st, ms, cts, nts) = (st', ms', cts', nts') ->
       joined st = joined st'.
   Proof.
     unfold end_query.
-    intuition.
-    repeat break_let.
-    find_apply_lem_hyp joined_preserved_by_try_rectify.
-    find_apply_lem_hyp joined_preserved_by_handle_delayed_queries.
-    simpl in *. (* simpl-ing through clear_query *)
-    now find_rewrite.
+    intros.
+    tuple_inversion.
+    tauto.
   Qed.
 
   Lemma joined_preserved_by_handle_stabilize : forall h src st q new_succ succ st' ms nts cts,
@@ -953,8 +947,8 @@ Section ChordProof.
     - find_apply_lem_hyp joined_preserved_by_end_query; auto.
   Qed.
 
-  Lemma joined_preserved_by_end_query_handle_rectify : forall h st p n st' ms nts cts,
-      end_query h (handle_rectify st p n) = (st', ms, nts, cts) ->
+  Lemma joined_preserved_by_end_query_handle_rectify : forall st p n st' ms nts cts,
+      end_query (handle_rectify st p n) = (st', ms, nts, cts) ->
       joined st = joined st'.
   Proof.
     unfold handle_rectify.
@@ -1839,216 +1833,6 @@ Section ChordProof.
       valid_ptr_timeout gst t0.
   Admitted.
 
-  Lemma handle_query_req_busy_definition :
-    forall src dst st msg st' ms newts clearedts,
-      handle_query_req_busy src dst st msg = (st', ms, newts, clearedts) ->
-      st' = delay_query st src msg /\
-      ms = [(src, Busy)] /\
-      clearedts = [] /\
-      ((delayed_queries st = [] /\ newts = [KeepaliveTick]) \/
-       (delayed_queries st <> [] /\ newts = [])).
-  Proof.
-    unfold handle_query_req_busy.
-    intros.
-    repeat break_match; tuple_inversion; tauto.
-  Qed.
-
-  Lemma handle_query_res_definition :
-    forall src dst st blank q p st' ms newts clearedts,
-      handle_query_res src dst st blank q p = (st', ms, newts, clearedts) ->
-      (request_payload p /\
-       st' = delay_query st src p /\
-       clearedts = [] /\
-       (delayed_queries st = [] /\
-        newts = [KeepaliveTick]) \/
-       (delayed_queries st <> [] /\
-        newts = [])) \/
-      (p = Busy /\
-       st' = st /\
-       newts = timeouts_in st /\
-       clearedts = timeouts_in st) \/
-      (exists n,
-          q = Rectify n /\
-          p = Pong /\
-          (exists pr,
-              pred st = Some pr /\
-              end_query dst (handle_rectify st pr n) = (st', ms, newts, clearedts)) \/
-          (pred st = None /\
-           end_query dst (update_pred st n, [], [], []) = (st', ms, newts, clearedts))) \/
-      (q = Stabilize /\
-       (exists new_succ succs,
-           p = GotPredAndSuccs (Some new_succ) succs /\
-           handle_stabilize dst (make_pointer src) st q new_succ succs = (st', ms, newts, clearedts)) \/
-       (exists succs,
-           p = GotPredAndSuccs None succs /\
-           end_query dst (st, [], [], []) = (st', ms, newts, clearedts))) \/
-      (exists new_succ,
-          q = Stabilize2 new_succ /\
-          exists succs,
-            p = GotSuccList succs /\
-            end_query dst (update_succ_list st (make_succs SUCC_LIST_LEN new_succ succs),
-                           [(addr_of new_succ, Notify)], [], []) = (st', ms, newts, clearedts)) \/
-      (exists k,
-          q = Join k /\
-          (exists bestpred,
-              p = GotBestPredecessor bestpred /\
-              clearedts = [Request src (GetBestPredecessor (make_pointer dst))] /\
-              st' = st /\
-              (addr_of bestpred = src /\
-               ms = [(src, GetSuccList)] /\
-               newts = [Request src GetSuccList]) \/
-              (addr_of bestpred <> src /\
-               ms = [(addr_of bestpred, (GetBestPredecessor (make_pointer dst)))] /\
-               newts = [Request (addr_of bestpred) (GetBestPredecessor (make_pointer dst))])) \/
-          (p = GotSuccList [] /\
-           end_query dst (st, [], [], []) = (st', ms, newts, clearedts)) \/
-          (exists new_succ rest,
-              p = GotSuccList (new_succ :: rest) /\
-              start_query (addr_of new_succ) st (Join2 new_succ) = (st', ms, newts, clearedts))) \/
-      (exists new_succ succs,
-          q = Join2 new_succ /\
-          p = GotSuccList succs /\
-          add_tick (end_query dst (update_for_join st (make_succs SUCC_LIST_LEN new_succ succs), [], [], [])) = (st', ms, newts, clearedts)) \/
-      st' = st /\ ms = [] /\ newts = [] /\ clearedts = [].
-  Proof.
-    unfold handle_query_res.
-    intros.
-    repeat break_match; try tuple_inversion; try tauto.
-    - right. right. left. eexists. intuition eauto.
-    - intuition eauto.
-    - intuition eauto.
-    - intuition eauto.
-    - intuition eauto.
-    - do 5 right. left.
-      exists p0. left. firstorder.
-      eexists; intuition eauto.
-    - do 5 right. left.
-      exists p0. intuition eauto.
-    - repeat find_rewrite.
-      do 5 right. left.
-      exists p0. right.
-      intuition.
-    - do 5 right. left.
-      exists p0.
-      intuition eauto.
-    - intuition eauto.
-  Qed.
-
-  Lemma recv_handler_definition :
-    forall src dst st p st' ms newts clearedts,
-      recv_handler src dst st p = (st', ms, newts, clearedts) ->
-      p = Ping /\
-      st' = st /\
-      ms = [(src, Pong)] /\
-      newts = [] /\
-      clearedts = [] \/
-
-      p = Notify /\
-      st' = set_rectify_with st (make_pointer src) /\
-      ms = [] /\
-      newts = [] /\
-      clearedts = [] \/
-
-      (exists qd q qm,
-          cur_request st = Some (qd, q, qm) /\
-          (request_payload p /\
-           st' = delay_query st src p /\
-           clearedts = [] /\
-           (delayed_queries st = [] /\
-            newts = [KeepaliveTick]) \/
-           (delayed_queries st <> [] /\
-            newts = [])) \/
-          (p = Busy /\
-           st' = st /\
-           newts = timeouts_in st /\
-           clearedts = timeouts_in st) \/
-          (exists n,
-              q = Rectify n /\
-              p = Pong /\
-              (exists pr,
-              pred st = Some pr /\
-              end_query dst (handle_rectify st pr n) = (st', ms, newts, clearedts)) \/
-          (pred st = None /\
-           end_query dst (update_pred st n, [], [], []) = (st', ms, newts, clearedts))) \/
-      (q = Stabilize /\
-       (exists new_succ succs,
-           p = GotPredAndSuccs (Some new_succ) succs /\
-           handle_stabilize dst (make_pointer src) st q new_succ succs = (st', ms, newts, clearedts)) \/
-       (exists succs,
-           p = GotPredAndSuccs None succs /\
-           end_query dst (st, [], [], []) = (st', ms, newts, clearedts))) \/
-      (exists new_succ,
-          q = Stabilize2 new_succ /\
-          exists succs,
-            p = GotSuccList succs /\
-            end_query dst (update_succ_list st (make_succs SUCC_LIST_LEN new_succ succs),
-                           [(addr_of new_succ, Notify)], [], []) = (st', ms, newts, clearedts)) \/
-      (exists k,
-          q = Join k /\
-          (exists bestpred,
-              p = GotBestPredecessor bestpred /\
-              clearedts = [Request src (GetBestPredecessor (make_pointer dst))] /\
-              st' = st /\
-              (addr_of bestpred = src /\
-               ms = [(src, GetSuccList)] /\
-               newts = [Request src GetSuccList]) \/
-              (addr_of bestpred <> src /\
-               ms = [(addr_of bestpred, (GetBestPredecessor (make_pointer dst)))] /\
-               newts = [Request (addr_of bestpred) (GetBestPredecessor (make_pointer dst))])) \/
-          (p = GotSuccList [] /\
-           end_query dst (st, [], [], []) = (st', ms, newts, clearedts)) \/
-          (exists new_succ rest,
-              p = GotSuccList (new_succ :: rest) /\
-              start_query (addr_of new_succ) st (Join2 new_succ) = (st', ms, newts, clearedts))) \/
-      (exists new_succ succs,
-          q = Join2 new_succ /\
-          p = GotSuccList succs /\
-          add_tick (end_query dst (update_for_join st (make_succs SUCC_LIST_LEN new_succ succs), [], [], [])) = (st', ms, newts, clearedts)) \/
-      st' = st /\ ms = [] /\ newts = [] /\ clearedts = []
-      ) \/
-
-      (cur_request st = None /\
-       st' = st /\
-       clearedts = [] /\
-       newts = [] /\
-       ((exists h,
-           p = GetBestPredecessor h /\
-           ms = [(src, GotBestPredecessor (best_predecessor (ptr st) (succ_list st) (id_of h)))]) \/
-       (p = GetSuccList /\
-        ms = [(src, GotSuccList (succ_list st))]) \/
-       (p = GetPredAndSuccs /\
-        ms = [(src, GotPredAndSuccs (pred st) (succ_list st))]))) \/
-
-      st = st' /\ ms = [] /\ newts = [] /\ clearedts = [].
-  Proof.
-    unfold recv_handler.
-    intros.
-    break_if.
-    - unfold handle_safe_msg, handle_notify in *.
-      find_apply_lem_hyp safe_msgs; break_or_hyp;
-      tuple_inversion; intuition.
-    - repeat break_match.
-      + find_eapply_lem_hyp handle_query_req_busy_definition.
-        repeat break_and.
-        find_apply_lem_hyp is_request_same_as_request_payload.
-        do 2 right. left.
-        repeat eexists; left; split; eauto.
-        repeat split.
-        repeat break_and.
-        break_or_hyp; intuition eauto.
-      + find_eapply_lem_hyp handle_query_res_definition.
-        do 2 right. left.
-        repeat eexists; intuition eauto.
-      + unfold handle_query_req in *.
-        break_match;
-          try discriminate;
-          repeat find_inversion;
-          try tuple_inversion;
-          intuition eauto.
-      + tuple_inversion; intuition eauto.
-      + tuple_inversion; intuition eauto.
-  Qed.
-
   Lemma In_timeouts_in :
     forall t st,
       In t (timeouts_in st) ->
@@ -2080,118 +1864,6 @@ Section ChordProof.
     end; congruence.
   Qed.
 
-  Lemma try_rectify_definition :
-    forall h st ms nts cts st' ms' nts' cts',
-      try_rectify h (st, ms, nts, cts) = (st', ms', nts', cts') ->
-      (joined st = true /\
-       (exists new,
-           rectify_with st = Some new /\
-           (exists x sq_ms sq_nts sq_cts,
-               pred st = Some x /\
-               start_query h (clear_rectify_with st) (Rectify new) = (st', sq_ms, sq_nts, sq_cts) /\
-               ms' = ms ++ sq_ms /\
-               nts' = nts ++ sq_nts /\
-               cts' = cts ++ sq_cts) \/
-           (pred st = None /\
-            st' = clear_rectify_with (update_pred st new) /\
-            ms' = ms /\
-            nts' = nts /\
-            cts' = cts))) \/
-      ((joined st = false \/ rectify_with st = None) /\
-       (st', ms', nts', cts') = (st, ms, nts, cts)).
-  Proof.
-    unfold try_rectify.
-    intros.
-    repeat break_match; tuple_inversion.
-    - left.
-      split; eauto.
-      intuition eauto.
-      exists p.
-      left.
-      intuition eauto.
-      repeat eexists; intuition eauto.
-    - left.
-      split; try tauto.
-      eexists; right; split; eauto.
-    - tauto.
-    - tauto.
-  Qed.
-
-  Lemma start_query_definition : 
-    forall h st k st' ms nts cts,
-      start_query h st k = (st', ms, nts, cts) ->
-      (exists dst msg,
-          make_request hash h st k = Some (dst, msg) /\
-          st' = update_query st dst k msg /\
-          ms = [(addr_of dst, msg)] /\
-          nts = [Request (addr_of dst) msg] /\
-          cts = timeouts_in st) \/
-      (make_request hash h st k = None /\
-       st' = st /\
-       ms = [] /\
-       ms = [] /\
-       nts = [] /\
-       cts = []).
-  Proof.
-    unfold start_query.
-    intros.
-    repeat break_match; tuple_inversion; try tauto.
-    left; repeat eexists.
-  Qed.
-
-  Lemma handle_delayed_queries_definition :
-    forall h st st' ms nts cts,
-     handle_delayed_queries h st = (st', ms, nts, cts) ->
-     st' = clear_delayed_queries st /\
-     ms = concat (map (handle_delayed_query h st) (delayed_queries st)) /\
-     nts = [] /\
-     cts = [KeepaliveTick].
-  Proof.
-    unfold handle_delayed_queries.
-    intros.
-    tuple_inversion.
-    intuition eauto.
-  Qed.
-
-  Lemma end_query_definition :
-    forall h st ms newts clearedts st' ms' newts' clearedts',
-      end_query h (st, ms, newts, clearedts) = (st', ms', newts', clearedts') ->
-      exists st'' ms'',
-        handle_delayed_queries h (clear_query st) = (st'', ms'', [], [KeepaliveTick]) /\
-        try_rectify h (st'', ms'' ++ ms, newts, timeouts_in st ++ [KeepaliveTick] ++ clearedts) = (st', ms', newts', clearedts').
-  Proof.
-    unfold end_query.
-    intros.
-    repeat break_let.
-    find_apply_lem_hyp handle_delayed_queries_definition.
-    repeat (break_and || break_or_hyp || break_exists).
-    subst_max.
-    repeat eexists; eauto.
-  Qed.
-
-  Lemma handle_rectify_definition :
-    forall st my_pred notifier st' ms nts cts,
-      handle_rectify st my_pred notifier = (st', ms, nts, cts) ->
-      ms = [] /\
-      nts = [] /\
-      cts = [] /\
-      (between (id_of my_pred) (id_of notifier) (id_of (ptr st)) /\
-       st' = update_pred st notifier \/
-       ~ between (id_of my_pred) (id_of notifier) (id_of (ptr st)) /\
-       st' = st).
-  Proof.
-    unfold handle_rectify.
-    intros.
-    rewrite between_between_bool_equiv.
-    break_if; tuple_inversion; firstorder.
-  Qed.
-
-  Ltac expand_def :=
-    repeat (try break_or_hyp; try break_and; try break_exists);
-    subst_max;
-    try tuple_inversion;
-    try (exfalso; tauto).
-
   Lemma valid_ptrs_global_recv_handler :
     forall gst xs m ys d st ms newts clearedts,
       valid_ptrs_global gst ->
@@ -2203,110 +1875,6 @@ Section ChordProof.
       forall t, In t newts ->
            valid_ptr_timeout gst t.
   Proof.
-    intros.
-    find_apply_lem_hyp recv_handler_definition.
-    find_apply_lem_hyp valid_ptrs_global_elim; break_and.
-    assert (valid_ptr_payload gst (snd (snd m))).
-    { apply valid_ptrs_net_elim_snd_snd;
-      try find_rewrite; auto with datatypes. }
-    expand_def.
-    - find_apply_lem_hyp in_inv.
-      break_or_hyp; try (exfalso; auto with *; fail).
-      constructor.
-    - find_apply_lem_hyp In_timeouts_in.
-      break_exists; break_and; subst_max.
-      constructor.
-      assert (valid_ptrs_state gst d).
-      { pose proof (H6 (fst (snd m))).
-        find_eapply_lem_hyp lift_pred_opt_Some_elim; eauto. }
-      find_apply_lem_hyp valid_ptrs_state_elim.
-      find_rewrite.
-      inv H10.
-      simpl in *; tauto.
-    - break_and.
-      destruct (handle_rectify _ _ _) eqn:H_rectify.
-      repeat destruct p.
-      find_eapply_lem_hyp end_query_definition.
-      break_exists.
-      break_and.
-      find_apply_lem_hyp try_rectify_definition.
-      expand_def; try (exfalso; tauto).
-      + find_apply_lem_hyp start_query_definition.
-        find_apply_lem_hyp handle_rectify_definition.
-        expand_def;
-          try (find_apply_lem_hyp in_inv;
-                break_or_hyp; try (exfalso; eauto using in_nil; fail)).
-        * constructor.
-          simpl in *.
-          break_match; find_inversion || congruence.
-          constructor.
-        * constructor.
-          simpl in *.
-          break_match; find_inversion || congruence.
-          constructor.
-      + find_eapply_lem_hyp handle_rectify_definition.
-        expand_def; exfalso; tauto.
-      + find_eapply_lem_hyp handle_rectify_definition.
-        expand_def; exfalso; tauto.
-      + find_eapply_lem_hyp handle_rectify_definition.
-        expand_def; exfalso; tauto.
-    - find_eapply_lem_hyp end_query_definition; expand_def.
-      find_eapply_lem_hyp try_rectify_definition; expand_def;
-      try (exfalso; tauto).
-      + simpl in *.
-        find_eapply_lem_hyp start_query_definition; expand_def;
-        simpl in *; try break_or_hyp; try (exfalso; tauto).
-        break_match.
-        * find_inversion.
-          do 2 constructor.
-        * discriminate.
-    - admit. (* handle_stabilize *)
-    - find_eapply_lem_hyp end_query_definition.
-      expand_def.
-      find_eapply_lem_hyp try_rectify_definition.
-      expand_def.
-      simpl in *.
-      find_eapply_lem_hyp start_query_definition.
-      expand_def.
-      simpl in *; break_or_hyp; try (exfalso; tauto).
-      break_match; try discriminate.
-      repeat find_inversion.
-      do 2 constructor.
-    - find_eapply_lem_hyp end_query_definition.
-      expand_def.
-      find_eapply_lem_hyp try_rectify_definition.
-      expand_def.
-      simpl in *.
-      find_eapply_lem_hyp start_query_definition.
-      expand_def.
-      simpl in *; break_or_hyp; try (exfalso; tauto).
-      break_match; try discriminate.
-      repeat find_inversion.
-      do 2 constructor.
-    - simpl in *; break_or_hyp; try (exfalso; tauto).
-      do 2 constructor.
-    - simpl in *; break_or_hyp; try (exfalso; tauto).
-      do 2 constructor.
-      apply valid_ptr_intro.
-      + apply make_pointer_valid.
-      + assumption.
-    - find_eapply_lem_hyp end_query_definition.
-      expand_def.
-      find_eapply_lem_hyp try_rectify_definition.
-      expand_def.
-      simpl in *.
-      find_eapply_lem_hyp start_query_definition.
-      expand_def.
-      simpl in *; break_or_hyp; try (exfalso; tauto).
-      break_match; try discriminate.
-      repeat find_inversion.
-      do 2 constructor.
-    - find_eapply_lem_hyp start_query_definition.
-      expand_def.
-      simpl in *; break_or_hyp; try (exfalso; tauto).
-      repeat find_inversion.
-      do 2 constructor.
-    - admit. (* add_tick on end_query *)
   Admitted.
 
   Lemma valid_ptrs_global_timeouts :
